run_yield_1 adequacy WIP

theories/examples/run_yield_1_adequacy.v
@@ -5,15 +5,7 @@ From iris.proofmode Require Import tactics.
 From iris.base_logic Require Import invariants na_invariants.
 From iris.bi Require Import big_op.
 
-Section Adequacy.
-  Context (Σ: gFunctors).
-  Context {inv_preG : invGS Σ}.
-  Context {nainv_preG : na_invG Σ}.
-  Context {vm_preG: gen_VMPreG Addr VMID Word reg_name PID transaction_type Σ}.
-  Context {tokG: tokG Σ}.
-
-  (* exec_mode of all VMs *)
-  Definition run_vms (ms: list exec_mode) (z i: VMID):=
+ Definition run_vms (ms: list exec_mode) (z i: VMID):=
     ms !! (fin_to_nat i) = Some ExecI ∧
     ms !! (fin_to_nat z) = Some ExecI ∧
     ∀ v , (v ≠ (fin_to_nat z) ∧ v ≠ (fin_to_nat i) -> ms !! v = Some HaltI).
@@ -34,53 +26,65 @@ Section Adequacy.
     (dom (gset handle) (get_transactions σ).1) ## ((get_transactions σ).2) ∧
     (get_transactions σ).2 ≠ ∅.
 
-  Definition is_initial_config (σ: state) (ms: list exec_mode):=
+  Definition is_initial_config (σ: state) (ms: list exec_mode) (φs : list (exec_mode -> Prop )):=
     ∃ (z i:VMID), (fin_to_nat z) = 0 ∧ z ≠ i ∧
                   (get_current_vm σ) = z ∧
+                  φs !! 0 = Some (λ m ,  m = HaltI ) ∧
+                  (∀ (v:nat) , v ≠ 0 -> φs !! v = Some (λ _, True)) ∧
     ∃ (p1 p2: PID), p1 ≠ p2 ∧
                   (run_vms ms z i) ∧
                   (mem_layout σ z i p1 p2) ∧
                   (reg σ z i p1 p2) ∧
                   transactions σ.
 
+Section Adequacy.
+  Context {nainv_preG : na_invG gen_VMΣ}.
+  Context {vm_preG: gen_VMPreG Addr VMID Word reg_name PID transaction_type gen_VMΣ}.
+  Context {tokG: tokG gen_VMΣ}.
 
-
-
-  Lemma run_yield_1_adequacy' (σ σ': state)  (ms ms': list exec_mode):
+  (* exec_mode of all VMs *)
+   About adequate.
+  Lemma run_yield_1_adequacy' (σ : state) (ms : list exec_mode) φs:
     (* we need assumptions to be able to allocate resources *)
     (* with these resources, we apply the specification and get the wptp *)
     (* along with some other stuff, then it should be enough to apply the adequacy theorem *)
-    (is_initial_config σ ms) ->
-    rtc machine.step (ms, σ) (ms', σ') →
+    (is_initial_config σ ms φs) ->
+    adequate ms σ ((λ φ, λ v _, φ v)<$> φs).
     (* φ : vm 0 is scheduled but halted *)
-    ((* scheduled σ' z ∧ *)  ms' !! 0 = Some HaltI).
   Proof.
-    intros Hinit Hstep.
-    pose proof (wp_invariance Σ hyp_machine ms σ ms' σ') as WPI;cbn in WPI.
-    apply WPI. 2: assumption.
-    clear WPI.
+    intros Hinit.
+    eapply (wp_adequacy gen_VMΣ).
+    { apply _. }
+    (* apply adequate_alt. *)
+    (* intros ms' σ' Hstep. *)
+    (* apply rtc_nsteps_1 in Hstep as [n Hstep]. *)
+    (* apply wp_strong_adequacy *)
+    (* pose proof (wp_adequacy Σ hyp_machine ms σ  ) as WPI;cbn in WPI. *)
+    (* apply WPI. 2: assumption. *)
+    (* clear WPI. *)
     intro Hinv.
+    iIntros.
 
     destruct Hinit as ( z & i & Heqz & Hneq & Hcur & Hinit).
-    iMod (@na_alloc Σ nainv_preG) as (nainv_gname) "Hna".
-    iMod (@gen_token_alloc Σ vm_preG z) as (token_gname) "[Hσtok Htok]".
-    iMod (@gen_mem_alloc Σ vm_preG (get_mem σ)) as (mem_gname) "[Hσmem Hmem]".
-    iMod (@gen_reg_alloc Σ vm_preG (get_reg_gmap σ)) as (reg_gname) "[Hσreg Hreg]".
+    iMod (na_alloc) as (nainv_gname) "Hna".
+    iMod (gen_token_alloc z) as (token_gname) "[Hσtok Htok]".
+    iMod (gen_mem_alloc (get_mem σ)) as (mem_gname) "[Hσmem Hmem]".
+    iMod (gen_reg_alloc (get_reg_gmap σ)) as (reg_gname) "[Hσreg Hreg]".
     iMod (gen_tx_alloc (get_tx_agree σ)) as (tx_gname) "[Hσtx _]".
     { apply get_txrx_auth_agree_valid. }
     iMod (gen_rx_agree_alloc (get_rx_agree σ)) as (rx_agree_gname) "[Hσrx_a _]".
     { apply get_txrx_auth_agree_valid. }
     iMod (gen_rx_option_alloc (get_rx_gmap σ)) as (rx_option_gname) "[Hσrx_o _]".
     iMod (gen_pagetable_alloc (get_owned_gmap σ)) as (own_gname) "[Hσown _]".
-    iMod (@gen_pagetable_alloc Σ vm_preG (get_access_gmap σ)) as (access_gname) "[Hσaccess Haccess]".
+    iMod (gen_pagetable_alloc (get_access_gmap σ)) as (access_gname) "[Hσaccess Haccess]".
     iMod (gen_pagetable_alloc (get_excl_gmap σ)) as (excl_gname) "[Hσexcl _]".
     iMod (gen_trans_alloc (get_trans_gmap σ)) as (trans_gname) "[Hσtrans _]".
     iMod (gen_hpool_alloc (get_hpool_gset σ)) as (hpool_gname) "[Hσhpool _]".
     iMod (gen_retri_alloc (get_retri_gmap σ)) as (retri_gname) "[Hσretri _]".
-    pose vmG := GenVMG Σ vm_preG inv_preG nainv_preG nainv_gname token_gname mem_gname reg_gname tx_gname
+    pose vmG := GenVMG gen_VMΣ vm_preG Hinv nainv_preG nainv_gname token_gname mem_gname reg_gname tx_gname
     rx_agree_gname rx_option_gname own_gname access_gname excl_gname trans_gname hpool_gname retri_gname.
 
-    destruct Hinit as (p1 & p2 & Hpne & Hms & Hmem & Hreg & Htrans ).
+    destruct Hinit as (Hφz & Hφs & p1 & p2 & Hpne & Hms & Hmem & Hreg & Htrans ).
     destruct Hreg as (Hreg1 & Hreg2).
     destruct Hreg1 as (r0_ & r1_ & Hreg1).
     destruct Hreg2 as (r0_'  & Hreg2).
@@ -100,14 +104,36 @@ Section Adequacy.
 
     iDestruct ((big_sepM_subseteq _ (get_reg_gmap σ) {[(PC, z):= (of_pid p1); (R0, z) := r0_;
                                  (R1,z):= r1_ ; (PC,i):= (of_pid p2); (R0,i):= r0_' ]}) with "Hreg" ) as "Hreg";eauto.
-    { admit. }
+    { rewrite /get_reg_gmap.
+      apply map_subseteq_spec.
+      intros.
+      apply elem_of_list_to_map.
+      { admit. }
+      apply elem_of_list_In.
+      apply in_flat_map.
+      exists i0.2.
+      split.
+      apply in_list_of_vmids.
+      apply in_map_iff.
+      exists (i0.1, x).
+      split.
+      destruct i0.
+      cbn.
+      done.
+      apply elem_of_list_In.
+      apply elem_of_map_to_list.
+      destruct i0.
+      cbn.
+      admit.
+      (* v = z ∨ v = i *)
+      }
 
 
     destruct Hmem as (Hacc1 & Hacc2 & Hmem).
     iDestruct ((gen_pagetable_split_2 z i) with "[Haccess]") as "(Haccessz & Haccessi & _)";eauto.
     set (sacc1 := (get_pagetable_gset σ z (λ pt : page_table, pt.2) is_accessible)) in *.
     set (sacc2 := (get_pagetable_gset σ i (λ pt : page_table, pt.2) is_accessible)) in *.
-    pose proof (@run_yield_1_spec Σ vmG tokG nroot z i 1 1 p1 p2 sacc1 sacc2 r0_ r1_ r0_' Heqz  Hneq Hpne)
+    pose proof (@run_yield_1_spec gen_VMΣ vmG tokG nroot z i 1 1 p1 p2 sacc1 sacc2 r0_ r1_ r0_' Heqz  Hneq Hpne)
       as HSpec.
 
     iDestruct (HSpec with "[Hmem Htok Hreg Haccessz Haccessi Hna]") as "HWPs";eauto.
@@ -192,71 +218,145 @@ Section Adequacy.
     }
     }
 
+    iMod "HWPs" as "[HWPz HWPi]".
+    iModIntro.
+
+    rewrite /run_vms in Hms.
+    destruct Hms as (Hi& Hz & Hrest).
+    destruct ms.
+    done.
+    destruct φs.
+    done.
+    cbn in Hφz.
+    inversion Hφz.
+      rewrite Heqz /= in Hz.
+      inversion Hz;subst e.
+     iSplitL "HWPz".
+     rewrite Heqz.
+     iApply (wp_mono with "HWPz") .
+     iIntros (k) "[? ?]".
+     iFrame.
+     destruct (fin_to_nat i) eqn:Heqni.
+     exfalso.
+     apply Hneq.
+     apply fin_to_nat_inj.
+     rewrite Heqni Heqz //.
+     assert (∃ l1 l2, ms = l1 ++ [ExecI] ++ l2).
+     destruct ms.
+     done.
+     clear HSpec Hrest Heqni.
+     cbn in Hi.
+     cbn in Hφs.
+     generalize dependent n.
+     generalize dependent e.
+     induction ms.
+     intros.
+     destruct n.
+    cbn in Hi.
+    inversion Hi.
+    exists [], [].
+    cbn.
+    done.
+    cbn in Hi.
+    inversion Hi.
+    intros.
+    destruct n.
+    cbn in Hi.
+    inversion Hi.
+    exists [], (a::ms).
+    cbn;done.
+    cbn in Hi.
+    apply IHms in Hi.
+    destruct Hi.
+    destruct H.
+    exists (e::x), x0.
+    rewrite H.
+    cbn;done.
+
+    destruct H.
+    destruct H.
+    rewrite H.
+    rewrite H in Hi.
+    rewrite !big_opL_app.
+    cbn.
+    cbn in Hi.
+    destruct (decide (n = length x)).
+    iSplitR.
+    {  iApply big_sepL_intro.
+    iModIntro.
+    iIntros.
+    pose proof (Hrest (S k)).
+    rewrite Heqz in H1.
+    rewrite H in H1.
+    cbn in H1.
+    assert (S k ≠ 0 ∧ S  k ≠ S n).
+    split.
+    done.
+    rewrite e.
+    apply lookup_lt_Some in H0.
+    lia.
+    apply H1 in H2.
+    apply (lookup_app_l_Some _ (ExecI :: x0) ) in H0.
+    rewrite H2 in H0.
+    inversion H0.
+    iApply wp_terminated';eauto.
+    }
     iSplitL.
-    iAssert ( WP ExecI
-             @ z {{ m, ⌜m = HaltI⌝ ∗ program (program1 i) p1 ∗ A@z:={1}[sacc1]  ∗
-                PC @@ z ->r (p1 ^+ length (program1 i))%f }}  )%I as "Hwp".
-    { admit. }
+    iSplitL;[|done].
+    assert (n = length x + 0). rewrite e. lia.
+    rewrite H0.
+    iApply (wp_mono  with "HWPi").
+    iIntros.
+    done.
+
     iApply big_sepL_intro.
-
-
-    (* Unset Printing Notations. *)
-    (* cannot eliminate fupd, don't know why.... *)
-    (* iMod "HWPs". *)
-    (* iIntros (v m Hvm). *)
-    admit.
+    iModIntro.
+    iIntros.
+    pose proof (Hrest (S (length x + S k))).
+    rewrite Heqz in H1.
+    rewrite H in H1.
+    cbn in H1.
+    assert (S (length x + S k) ≠ 0 ∧ S (length x + S k) ≠ S n).
+    split.
+    done.
+    rewrite e.
+    lia.
+    apply H1 in H2.
+    apply lookup_app_Some in H2.
+    destruct H2.
+    apply lookup_lt_Some in H2.
+    lia.
+    destruct H2.
+    assert (length x + S k - length x = S k).
+    lia.
+    rewrite H4 in H3.
+    cbn in H3.
+    rewrite H3 in H0.
+    inversion H0.
+    iApply wp_terminated';eauto.
+    rewrite H in Hrest.
+    cbn in Hrest.
+    pose proof (Hrest (S (length x))).
+    assert (S (length x ) ≠ z ∧ S (length x) ≠ S n).
+    split. lia. lia.
+    apply H0 in H1.
+    cbn in H1.
+    apply lookup_app_Some in H1.
+    destruct H1.
+    apply lookup_lt_Some in H1.
+    lia.
+    destruct H1.
+    assert (length x - length x = 0). lia.
+    rewrite H3 in H2.
+    cbn in H2.
+    inversion H2.
 
     iModIntro.
 
+    iIntros.
+    iExists ⊤.
+    iModIntro.
 
-    (* [∗ list] WP -> WP @z ∗ WP @i *)
-    (* rewrite /run_vms in Hms. *)
-    (* iAssert *)
-    (*   (WP ExecI @ z {{ _, True }} ∗ WP ExecI @ i {{ _, True }} -∗ ([∗ list] id↦e ∈ ms, WP e @ id {{ _, True }}))%I as "Hwpimp". *)
-    (* { iIntros "[Hz Hi]". *)
-    (*   destruct Hms as (Hi& Hz & Hrest). *)
-    (*   destruct ms. *)
-    (*   done. *)
-    (*   rewrite Heqz /= in Hz. *)
-    (*   cbn. *)
-    (*   inversion Hz;subst e. *)
-    (*   rewrite Heqz. *)
-    (*   iFrame. *)
-    (*   iInduction ms as  [m | m] "IH". *)
-    (*   - done. *)
-    (*   - destruct (decide ((fin_to_nat i) = 1)). *)
-    (*     cbn. *)
-    (*     rewrite e // in Hi. *)
-    (*     simplify_list_eq. *)
-    (*     rewrite e. *)
-    (*     iFrame. *)
-    (*     iClear "IH". *)
-    (*     iInduction ms as  [m | m] "IH". *)
-    (*     + done. *)
-    (*     + cbn. *)
-    (*       assert (m= HaltI). *)
-    (*       assert (2 ≠ fin_to_nat (get_current_vm σ) ∧ 2 ≠ (fin_to_nat i)). *)
-    (*       rewrite Heqz;lia. *)
-    (*       pose proof (Hrest 2 H). *)
-    (*       cbn in H0. *)
-    (*       inversion H0;done. *)
-    (*       rewrite H. *)
-    (*       iSplitL. *)
-    (*       iApply wp_terminated';eauto. *)
-    (*       (* cannot apply induction hypothesis *) *)
-    (*       admit. *)
-    (*     + cbn. *)
-    (*       assert (1 ≠ fin_to_nat z ∧ 1 ≠ (fin_to_nat i)). *)
-    (*       rewrite Heqz;lia. *)
-    (*       pose proof (Hrest 1 H). *)
-    (*       cbn in H0. *)
-    (*       inversion H0. *)
-    (*       iSplitR. *)
-    (*       iApply wp_terminated';eauto. *)
-    (*       admit. *)
-    (* } *)
-
-    (* apply adequacy theorem *)
-  Admitted.
+   Admitted.
 
 End Adequacy.
